midterm-project/solutions/distributed_system.s.dfy
@@ -7,28 +7,35 @@ include "protocol.i.dfy"
 // Before we get here, caller must define a type Message that we'll
 // use to instantiate network.s.dfy.
 
-datatype DistVars = DistVars(
-  hosts:map<HostId, HostVars>, network:NetVars<Message>)
+module DistributedSystem {
+  datatype Constants = Constants(
+    hostCount: int,
+    hosts:map<HostId, HostVars>)
 
-predicate WFVars(v:DistVars) {
-  // We don't lose track of any of the hosts.
-  && v.hosts.Keys == AllHosts()
-}
+  datatype Variables = Variables(
+    hosts:map<HostId, HostVars>,
+    network:NetVars<Message>)
 
-predicate DistInit(v:DistVars) {
-  && WFVars(v)
-  && (forall id :: HostInit(v.hosts[id], id))
-  && NetInit(v.network)
-}
+  predicate WFVars(v:Variables) {
+    // We don't lose track of any of the hosts.
+    && v.hosts.Keys == AllHosts()
+  }
 
-predicate NextStep(v:DistVars, v':DistVars, id:HostId, a:NetAction<Message>) {
-  && WFVars(v)
-  && WFVars(v')
-  && HostNext(id, v.hosts[id], v'.hosts[id], a)
-  && (forall other :: other != id ==> v'.hosts[other] == v.hosts[other])
-  && NetNext(v.network, v'.network, a)
-}
+  predicate DistInit(v:Variables) {
+    && WFVars(v)
+    && (forall id :: HostInit(v.hosts[id], id))
+    && NetInit(v.network)
+  }
 
-predicate DistNext(v:DistVars, v':DistVars) {
-  exists id, a :: NextStep(v, v', id, a)
+  predicate NextStep(v:Variables, v':Variables, id:HostId, a:NetAction<Message>) {
+    && WFVars(v)
+    && WFVars(v')
+    && HostNext(id, v.hosts[id], v'.hosts[id], a)
+    && (forall other :: other != id ==> v'.hosts[other] == v.hosts[other])
+    && NetNext(v.network, v'.network, a)
+  }
+
+  predicate DistNext(v:Variables, v':Variables) {
+    exists id, a :: NextStep(v, v', id, a)
+  }
 }
